Make lock and counter consistent with spawn.

heap_lang/lib/lock.v
@@ -18,18 +18,18 @@ Instance inGF_lockG `{H : inGFs heap_lang Σ lockGF} : lockG Σ.
 Proof. destruct H. split. apply: inGF_inG. Qed.
 
 Section proof.
-Context `{!heapG Σ, !lockG Σ}.
+Context `{!heapG Σ, !lockG Σ} (N : namespace).
 Local Notation iProp := (iPropG heap_lang Σ).
 
 Definition lock_inv (γ : gname) (l : loc) (R : iProp) : iProp :=
   (∃ b : bool, l ↦ #b ★ if b then True else own γ (Excl ()) ★ R)%I.
 
 Definition is_lock (l : loc) (R : iProp) : iProp :=
-  (∃ N γ, heapN ⊥ N ∧ heap_ctx ∧ inv N (lock_inv γ l R))%I.
+  (∃ γ, heapN ⊥ N ∧ heap_ctx ∧ inv N (lock_inv γ l R))%I.
 
 Definition locked (l : loc) (R : iProp) : iProp :=
-  (∃ N γ, heapN ⊥ N ∧ heap_ctx ∧
-          inv N (lock_inv γ l R) ∧ own γ (Excl ()))%I.
+  (∃ γ, heapN ⊥ N ∧ heap_ctx ∧
+        inv N (lock_inv γ l R) ∧ own γ (Excl ()))%I.
 
 Global Instance lock_inv_ne n γ l : Proper (dist n ==> dist n) (lock_inv γ l).
 Proof. solve_proper. Qed.
@@ -43,9 +43,9 @@ Global Instance is_lock_persistent l R : PersistentP (is_lock l R).
 Proof. apply _. Qed.
 
 Lemma locked_is_lock l R : locked l R ⊢ is_lock l R.
-Proof. rewrite /is_lock. iDestruct 1 as (N γ) "(?&?&?&_)"; eauto. Qed.
+Proof. rewrite /is_lock. iDestruct 1 as (γ) "(?&?&?&_)"; eauto. Qed.
 
-Lemma newlock_spec N (R : iProp) Φ :
+Lemma newlock_spec (R : iProp) Φ :
   heapN ⊥ N →
   heap_ctx ★ R ★ (∀ l, is_lock l R -★ Φ #l) ⊢ WP newlock #() {{ Φ }}.
 Proof.
@@ -54,13 +54,13 @@ Proof.
   iPvs (own_alloc (Excl ())) as (γ) "Hγ"; first done.
   iPvs (inv_alloc N _ (lock_inv γ l R) with "[-HΦ]") as "#?"; first done.
   { iIntros ">". iExists false. by iFrame. }
-  iPvsIntro. iApply "HΦ". iExists N, γ; eauto.
+  iPvsIntro. iApply "HΦ". iExists γ; eauto.
 Qed.
 
 Lemma acquire_spec l R (Φ : val → iProp) :
   is_lock l R ★ (locked l R -★ R -★ Φ #()) ⊢ WP acquire #l {{ Φ }}.
 Proof.
-  iIntros "[Hl HΦ]". iDestruct "Hl" as (N γ) "(%&#?&#?)".
+  iIntros "[Hl HΦ]". iDestruct "Hl" as (γ) "(%&#?&#?)".
   iLöb as "IH". wp_rec. wp_focus (CAS _ _ _)%E.
   iInv N as ([]) "[Hl HR]".
   - wp_cas_fail. iPvsIntro; iSplitL "Hl".
@@ -68,13 +68,13 @@ Proof.
     + wp_if. by iApply "IH".
   - wp_cas_suc. iPvsIntro. iDestruct "HR" as "[Hγ HR]". iSplitL "Hl".
     + iNext. iExists true; eauto.
-    + wp_if. iApply ("HΦ" with "[-HR] HR"). iExists N, γ; eauto.
+    + wp_if. iApply ("HΦ" with "[-HR] HR"). iExists γ; eauto.
 Qed.
 
 Lemma release_spec R l (Φ : val → iProp) :
   locked l R ★ R ★ Φ #() ⊢ WP release #l {{ Φ }}.
 Proof.
-  iIntros "(Hl&HR&HΦ)"; iDestruct "Hl" as (N γ) "(% & #? & #? & Hγ)".
+  iIntros "(Hl&HR&HΦ)"; iDestruct "Hl" as (γ) "(% & #? & #? & Hγ)".
   rewrite /release. wp_let. iInv N as (b) "[Hl _]".
   wp_store. iPvsIntro. iFrame "HΦ". iNext. iExists false. by iFrame.
 Qed.
